theories/TM/Hoare/HoareLegacy.v
@@ -1,0 +1,16 @@
+From Undecidability.TM Require Import TM Util.TM_facts HoareLogic HoareRegister.
+
+Lemma RealiseIntroAll sig F n X (P : forall _ _ _ _, Prop) (M : pTM sig F n):
+  (forall x, M ⊨ (fun tin '(yout, tout) => P x tin yout tout)) ->
+  M ⊨ (fun tin '(yout, tout) => forall (x:X), P x tin yout tout).
+Proof.
+  unfold Realise. intros. firstorder. 
+Qed.
+
+Lemma TerminatesInIntroEx sig n X (T : forall _ _ _, Prop) (M : TM sig n):
+  (forall x, M ↓ (fun tin k => T x tin k)) ->
+  M ↓ (fun tin k => exists (x:X), T x tin k).
+Proof.
+  unfold TerminatesIn. intros. firstorder. 
+Qed.
+
