theories/TM/Univ/LookupAssociativeListTM.v
@@ -2,6 +2,8 @@ From PslBase Require Import Bijection. (* [injective] *)
 From Undecidability Require Import ProgrammingTools.
 From Undecidability Require Import TM.Code.CompareValue.
 From Undecidability Require Import TM.Code.CasePair TM.Code.CaseList.
+From Undecidability.TM.Hoare Require Import Hoare HoareLegacy.
+
 
 Local Arguments plus : simpl never.
 Local Arguments mult : simpl never.
@@ -23,12 +25,6 @@ Section LookupAssociativeList.
     | nil => None
     | (x', y) :: xs' => if Dec (x = x') then Some y else lookup x xs'
     end.
-
-  (*
-  Local Instance retr_sigPair_sig : Retract (sigPair sigX sigY) sig := ComposeRetract _ _.
-  Local Instance retr_sigX_sig : Retract sigX sig := ComposeRetract _ _.
-  Local Instance retr_sigY_sig : Retract sigY sig := ComposeRetract _ _.
-*)
 
   Local Definition retr_sig_sigX : Retract sigX sig := _.
   Local Definition retr_sig_sigY : Retract sigY sig := _.
@@ -55,64 +51,7 @@ Section LookupAssociativeList.
               (*2*) CaseList_size1 (x',y) >> CasePair_size0 x' >> Reset_size y;
               (*3*) CasePair_size1 x' >> Reset_size x' |]
     | nil => [| ResetEmpty1_size; id; id; id|]
-    end.
-  
-
-  Definition Lookup_Step_Rel : pRel sig^+ (option bool) 4 :=
-    fun tin '(yout, tout) =>
-      forall (xs : list (X*Y)) (x : X) (s0 s1 s2 s3 : nat),
-        let size := Lookup_Step_size xs x in
-        tin[@Fin0] ≃(;s0) xs ->
-        tin[@Fin1] ≃(;s1) x ->
-        isVoid_size tin[@Fin2] s2 -> isVoid_size tin[@Fin3] s3 ->
-        match xs with
-        | nil => yout = Some false /\
-                isVoid_size tout[@Fin0] (size@>Fin0 s0) /\
-                tout[@Fin1] ≃(;size@>Fin1 s1) x /\
-                isVoid_size tout[@Fin2] (size@>Fin2 s2) /\ isVoid_size tout[@Fin3] (size@>Fin3 s3)
-        | (x', y) :: xs' =>
-          if Dec (x = x')
-          then yout = Some true /\
-               isVoid_size tout[@Fin0] (size@>Fin0 s0) /\
-               tout[@Fin1] ≃(;size@>Fin1 s1) y /\
-               isVoid_size tout[@Fin2] (size@>Fin2 s2) /\
-               isVoid_size tout[@Fin3] (size@>Fin3 s3)
-          else yout = None /\
-               tout[@Fin0] ≃(;size@>Fin0 s0) xs' /\
-               tout[@Fin1] ≃(;size@>Fin1 s1) x /\
-               isVoid_size tout[@Fin2] (size@>Fin2 s2) /\ isVoid_size tout[@Fin3] (size@>Fin3 s3)
-        end.
-
-  Lemma Lookup_Step_Realise : Lookup_Step ⊨ Lookup_Step_Rel.
-  Proof.
-    eapply Realise_monotone.
-    { unfold Lookup_Step. TM_Correct.
-      - eapply CaseList_Realise.
-      - apply CompareValues_Realise with (1 := cX_injective).
-      - apply MoveValue_Realise with (X := Y) (Y := X).
-      - apply Reset_Realise with (X := X).
-      - apply Reset_Realise with (X := list (X*Y)).
-      - apply Reset_Realise with (X := X).
-      - apply Reset_Realise with (X := Y).
-      - eapply RealiseIn_Realise. apply ResetEmpty1_Sem with (X := list (X*Y)).
-    }
-    {
-      intros tin (yout, tout) H. cbn. intros xs x s0 s1 s2 s3 HEncXS HEncX HRight2 HRight3. destruct H; TMSimp.
-      { (* CaseList -> Then *) rename H into HMatchList, H0 into HMatchPair, H2 into HCompare.
-        modpon HMatchList. destruct xs as [ | p xs']; modpon HMatchList; auto.
-        modpon HMatchPair. destruct p as [ x' y]; cbn in *.
-        destruct HCompare; TMSimp.
-        { (* CompareValue ~> Then *) rename H into HCompareValue, H1 into HReset2, H3 into HReset3, H5 into HReset0.
-          modpon HCompareValue. decide (x=x') as [ <- | H ]; auto.
-          modpon HReset2. modpon HReset3. modpon HReset0. repeat split; auto.
-        }
-        { (* CompareValue ~> Else *) rename H into HCompareValue, H1 into HReset3, H3 into HReset2.
-          modpon HCompareValue. decide (x=x') as [ <- | H ]; auto.
-          modpon HReset3. modpon HReset2. repeat split; auto. }
-      }
-      { (* CaseList ~> Else *) modpon H. destruct xs as [ | ]; auto; modpon H. modpon H1. cbn. repeat split; auto. }
-    }
-  Qed.
+    end.    
 
   Definition Lookup_Step_steps_Compare {sigX sigY : Type} {X : eqType} {Y : Type} {cX : codable sigX X} {cY : codable sigY Y} (x x' : X) (y : Y) (xs : list (X*Y)) :=
     if Dec (x=x')
@@ -127,61 +66,59 @@ Section LookupAssociativeList.
 
   Definition Lookup_Step_steps {sigX sigY : Type} {X : eqType} {Y : Type} {cX : codable sigX X} {cY : codable sigY Y} (xs : list (X*Y)) (x : X) :=
     1 + CaseList_steps xs + Lookup_Step_steps_CaseList xs x.
-    
-  Definition Lookup_Step_T : tRel sig^+ 4 :=
-    fun tin k =>
-      exists (xs : list (X*Y)) (x : X),
-        tin[@Fin0] ≃ xs /\
-        tin[@Fin1] ≃ x /\
-        isVoid tin[@Fin2] /\ isVoid tin[@Fin3] /\
-        Lookup_Step_steps xs x <= k.
 
-  Lemma Lookup_Step_Terminates : projT1 Lookup_Step ↓ Lookup_Step_T.
+  Lemma Lookup_Step_SpecT_space (xs : list (X*Y)) (x : X) (ss : Vector.t nat 4) :
+    TripleT
+      (tspec (withSpace (SpecVector [|Contains _ xs; Contains _ x; Void; Void|]) ss))
+      (Lookup_Step_steps xs x)
+      Lookup_Step
+      (fun yout =>
+         tspec (withSpace
+           (match yout, xs with
+            | Some false, nil => SpecVector [|Void; Contains _ x; Void; Void|]
+            | _, (x',y) :: xs' =>
+              match yout, (Dec (x=x') : bool) with
+              | Some true, true =>
+                SpecVector [|Void; Contains _ y; Void; Void|]
+              | None, false =>
+                SpecVector [|Contains _ xs'; Contains _ x; Void; Void|]
+              | _, _ => SpecFalse
+              end
+            | _, _ => SpecFalse
+            end) (appSize (Lookup_Step_size xs x) ss))).
   Proof.
-    eapply TerminatesIn_monotone.
-    { unfold Lookup_Step. TM_Correct.
-      - eapply CaseList_Realise.
-      - eapply CaseList_Terminates.
-      - apply CompareValues_Realise with (1 := cX_injective).
-      - apply CompareValues_TerminatesIn with (X := X).
-      - apply MoveValue_Realise with (X := Y) (Y := X).
-      - apply MoveValue_Terminates with (X := Y) (Y := X).
-      - apply Reset_Realise with (X := X).
-      - apply Reset_Terminates with (X := X).
-      - apply Reset_Terminates with (X := list (X*Y)).
-      - apply Reset_Realise with (X := X).
-      - apply Reset_Terminates with (X := X).
-      - apply Reset_Terminates with (X := Y).
-      - eapply RealiseIn_TerminatesIn. apply ResetEmpty1_Sem with (X := list (X*Y)).
-    }
-    {
-      intros tin k (xs&x&HEncXs&HEncX&HRight2&HRight3&Hk). cbn. unfold Lookup_Step_steps in Hk.
-      exists (CaseList_steps xs), (Lookup_Step_steps_CaseList xs x). repeat split; try lia. eauto. 
-      intros tmid_ yout (HCaseList&HCaseListInj); TMSimp_old. modpon HCaseList. unfold Lookup_Step_steps_CaseList in *.
-      destruct yout, xs as [ | p xs']; cbn in *; auto; modpon HCaseList.
-      { (* cons case *) destruct p as [x' y]; cbn in *.
-        exists (CasePair_steps x'), (1 + CompareValues_steps x x' + Lookup_Step_steps_Compare x x' y xs'). repeat split; try lia.
-        { hnf; eauto. cbn. eexists. split; simpl_surject; eauto. }
-        intros tmid0 [] (HCasePair&HCasePairInj); TMSimp. modpon HCasePair. cbn in *.
-        exists (CompareValues_steps x x'), (Lookup_Step_steps_Compare x x' y xs'). repeat split; try lia.
-        { hnf. cbn. do 2 eexists. repeat split; simpl_surject; eauto. }
-        intros tmid1 ymid1 (HCompare&HCompareInj); TMSimp_old. modpon HCompare. subst.
-        unfold Lookup_Step_steps_Compare in *. decide (x = x') as [ <- | HDec].
-        - exists (MoveValue_steps y x), (1 + Reset_steps x + Reset_steps xs'). repeat split; try lia.
-          { do 2 eexists; repeat split; eauto. }
-          intros tmid2 []. intros (HMove&HMoveInj); TMSimp_old. modpon HMove.
-          exists (Reset_steps x), (Reset_steps xs'). repeat split; try lia.
-          { hnf. eexists; repeat split; eauto. }
-          intros tmid3 [] (HReset&HResetInj); TMSimp. modpon HReset.
-          eexists. repeat split; eauto.
-        - exists (Reset_steps x'), (Reset_steps y). repeat split; try lia.
-          { eexists; repeat split; eauto.  }
-          intros tmid2 [] (HReset&HRestInj); TMSimp. modpon HReset.
-          eexists; repeat split; eauto.
-      }
-    }
+    unfold Lookup_Step. unfold Lookup_Step_size; cbn.
+    eapply If_SpecT with (k1 := CaseList_steps xs) (k2 := Lookup_Step_steps_CaseList xs x) (k3 := Lookup_Step_steps_CaseList xs x).
+    - hstep; cbn. apply CaseList_SpecT_size.
+    - (* First "Then"; we have [xs = (x',y) :: xs']. *)
+      cbn. destruct xs as [ | (x', y) xs']; cbn in *; auto.
+      hstep.
+      + (* CasePair *) cbn.
+        hstep; cbn. hstep; cbn. hstep; cbn. cbn. tspec_ext.
+      + cbn. intros _.
+        eapply If_SpecT with (k1 := CompareValues_steps x x') (k2 := Lookup_Step_steps_Compare x x' y xs') (k3 := Lookup_Step_steps_Compare x x' y xs').
+        * hsteps_cbn; cbn. apply CompareValue_SpecT_size with (X := X). assumption. cbn. tspec_ext.
+        * (* Second "Then"; we have [x=x'] *) decide (x=x') as [Hx | ]; cbn in *; auto.
+          hstep. (* Return *) hstep. (* Seq *)
+          -- (* MoveValue *) hstep; cbn. apply MoveValue_SpecT_size with (X := Y) (Y := X).
+          -- cbn. intros _. hstep. (* Seq *)
+             ++ (* Reset X *) hstep; cbn.  apply Reset_SpecT_space with (X := X).
+             ++ (* Reset Y *) cbn. intros _. hstep. cbn. apply Reset_SpecT_space with (X := list (X*Y)).
+             ++ reflexivity.
+          -- unfold Lookup_Step_steps_Compare. dec_pos (x=x'). lia.
+          -- cbn. intros _. tspec_ext.
+        * cbn. (* "Else": We have [x<>x'] *) decide (x=x') as [ | Hx]; cbn in *; auto.
+          hstep. hstep.
+          -- hstep. cbn. eapply Reset_SpecT_space with (X := X).
+          -- cbn. intros _. hstep. cbn. apply Reset_SpecT_space with (X := Y).
+          -- unfold Lookup_Step_steps_Compare. dec_neg (x=x'). reflexivity.
+          -- cbn. intros _. tspec_ext.
+        * intros tin ymid tmid H1 H2. cbn in *. destruct ymid; decide (x=x') as [Hx|Hx]; cbn in *; auto.
+      + cbn. lia.
+    - cbn. (* The top-most "Else": We have [xs=nil] *) destruct xs as [ | ]; cbn in *; auto.
+      hstep. hstep. cbn. eapply ResetEmpty1_SpecT_space with (X := list (X*Y)). reflexivity. cbn. eauto.
+    - (* Finall running time *) intros tin yout tout _ _. destruct yout; reflexivity.
   Qed.
-
 
   Definition Lookup_Loop := While Lookup_Step.
 
@@ -194,46 +131,7 @@ Section LookupAssociativeList.
       then Lookup_Step_size xs x
       else Lookup_Step_size xs x >>> Lookup_Loop_size xs' x
     end.
-  
-  
-  Definition Lookup_Loop_Rel : pRel sig^+ bool 4 :=
-    fun tin '(yout, tout) =>
-      forall (xs : list (X*Y)) (x : X) (s0 s1 s2 s3 : nat),
-        let size := Lookup_Loop_size xs x in
-        tin[@Fin0] ≃(;s0) xs ->
-        tin[@Fin1] ≃(;s1) x ->
-        isVoid_size tin[@Fin2] s2 -> isVoid_size tin[@Fin3] s3 ->
-        match yout, lookup x xs with
-        | true, Some y =>
-          isVoid_size tout[@Fin0] (size@>Fin0 s0) /\
-          tout[@Fin1] ≃(;size@>Fin1 s1) y /\
-          isVoid_size tout[@Fin2] (size@>Fin2 s2) /\
-          isVoid_size tout[@Fin3] (size@>Fin3 s3)
-        | false, None =>
-          isVoid_size tout[@Fin0] (size@>Fin0 s0) /\
-          tout[@Fin1] ≃(;size@>Fin1 s1) x /\
-          isVoid_size tout[@Fin2] (size@>Fin2 s2) /\
-          isVoid_size tout[@Fin3] (size@>Fin3 s3)
-        | _, _ => False
-        end.
-
-
-  Lemma Lookup_Loop_Realise : Lookup_Loop ⊨ Lookup_Loop_Rel.
-  Proof.
-    eapply Realise_monotone.
-    { unfold Lookup_Loop. TM_Correct. apply Lookup_Step_Realise. }
-    { apply WhileInduction; intros; cbn; intros xs x s0 s1 s2 s3 HEncXs HEncX HRight2 HRight3; cbn in *.
-      - modpon HLastStep. destruct xs as [ | (x'&y)]; cbn in *; modpon HLastStep; auto.
-        + inv HLastStep. auto.
-        + decide (x = x') as [ <- | HDec]; modpon HLastStep; inv HLastStep; auto.
-      - modpon HStar. destruct xs as [ | (x'&y)]; cbn in *; modpon HStar; try now inv HStar.
-        decide (x = x') as [ <- | HDec]; modpon HStar; try now inv HStar.
-        modpon HLastStep. auto.
-    }
-  Qed.
-
-  Local Arguments Lookup_Loop_size : simpl never.
-  
+    
 
   Fixpoint Lookup_Loop_steps {sigX sigY : Type} {X : eqType} {Y : Type} {cX : codable sigX X} {cY : codable sigY Y} (x : X) (xs : list (X*Y)) { struct xs } :=
     match xs with
@@ -243,33 +141,35 @@ Section LookupAssociativeList.
                       else 1 + Lookup_Step_steps xs x + Lookup_Loop_steps x xs'
     end.
 
-  Definition Lookup_Loop_T : tRel sig^+ 4 :=
-    fun tin k =>
-      exists (xs : list (X*Y)) (x : X),
-        tin[@Fin0] ≃ xs /\
-        tin[@Fin1] ≃ x /\
-        isVoid tin[@Fin2] /\ isVoid tin[@Fin3] /\
-        Lookup_Loop_steps x xs <= k.
-
-  Lemma Lookup_Loop_Terminates : projT1 Lookup_Loop ↓ Lookup_Loop_T.
+  Lemma Lookup_Loop_SpecT_space (xs : list (X*Y)) (x : X) (ss : Vector.t nat 4) :
+  TripleT
+    (tspec (withSpace (SpecVector [|Contains _ xs; Contains _ x; Void; Void|]) ss))
+    (Lookup_Loop_steps x xs) Lookup_Loop
+    (fun yout =>
+      tspec
+        (withSpace
+            match yout, lookup x xs with
+            | true, Some y => SpecVector [|Void; Contains _ y; Void; Void|]
+            | false,  None => SpecVector [|Void; Contains _ x; Void; Void|]
+            | _, _ => SpecFalse
+            end (appSize (Lookup_Loop_size xs x) ss))).
   Proof.
-    eapply TerminatesIn_monotone.
-    { unfold Lookup_Loop. TM_Correct.
-      - apply Lookup_Step_Realise.
-      - apply Lookup_Step_Terminates. }
-    { eapply WhileCoInduction; intros. destruct HT as (xs&x&HEncXs&HEncX&HRight2&HRight3&Hk).
-      exists (Lookup_Step_steps xs x). repeat split.
-      { hnf. do 2 eexists; repeat split; eauto. }
-      intros ymid tmid HStep. cbn in HStep. modpon HStep.
-      destruct xs as [ | (x'&y) xs']; modpon HStep; subst.
-      - cbn. auto.
-      - cbn in *. decide (x = x') as [ <- | ]; modpon HStep; subst.
-        + auto.
-        + exists (Lookup_Loop_steps x xs'). split; eauto.
-          hnf. do 2 eexists; repeat split; eauto.
-    }
+  unfold Lookup_Loop.
+  eapply While_SpecT with (P := fun '(xs, x, ss) => _) (Q := fun '(xs, x, ss) => _) (R := fun '(xs, x, ss) => _) (g := fun '(xs,x,ss) => _) (f := fun '(xs,x,ss) => _)
+                          (x := (xs,x,ss)); clear x xs ss; intros ((xs, x), ss).
+  - apply Lookup_Step_SpecT_space.
+  - intros [] tmid tout H1 H2.
+    destruct xs as [ | (x', y) xs']; cbn in *; auto.
+    + decide (x = x'); cbn in *; eauto.
+    + destruct xs as [ | (x', y) xs']; cbn in *; auto.
+  - cbn. intros tin tmid Htin Hmid.
+    destruct xs as [ | (x', y) xs']; cbn in *; auto.
+    decide (x = x'); cbn in *; eauto.
+    eexists (_, _, _); cbn. repeat split.
+    + eauto.
+    + reflexivity.
+    + eauto.
   Qed.
-
 
   Definition Lookup : pTM sig^+ bool 5 :=
     CopyValue _ @ [|Fin0; Fin4|];; Lookup_Loop @ [|Fin4; Fin1; Fin2; Fin3|].
@@ -278,6 +178,7 @@ Section LookupAssociativeList.
     ([|CopyValue_size xs|] @>> [|Fin4|]) >>>
     (Lookup_Loop_size xs x @>>[|Fin4; Fin1; Fin2; Fin3|]).
 
+  
   Definition Lookup_Rel : pRel sig^+ bool 5 :=
     fun tin '(yout, tout) =>
       forall (xs : list (X*Y)) (x : X) (s0 s1 s2 s3 s4 : nat),
@@ -301,19 +202,42 @@ Section LookupAssociativeList.
         | _, _ => False
         end.
 
-  Lemma Lookup_Realise : Lookup ⊨ Lookup_Rel.
-  Proof.
-    eapply Realise_monotone.
-    { unfold Lookup. TM_Correct.
-      - apply CopyValue_Realise with (X := list (X*Y)).
-      - apply Lookup_Loop_Realise. }
-    { intros tin (yout, tout) H. cbn. TMSimp. intros. modpon H. modpon H0. TMCrush; auto. all: repeat split; try rewrite !vector_tl_nth; auto. }
-  Qed.
-
 
   Definition Lookup_steps {sigX sigY : Type} {X : eqType} {Y : Type} {cX : codable sigX X} {cY : codable sigY Y} (x : X) (xs : list (X*Y)) :=
     1 + CopyValue_steps xs + Lookup_Loop_steps x xs.
 
+    Lemma Lookup_SpecT_space (xs : list (X*Y)) (x : X) (ss : Vector.t nat 5) :
+    TripleT
+      (tspec (withSpace (SpecVector [|Contains _ xs; Contains _ x; Void; Void; Void|]) ss))
+      (Lookup_steps x xs) Lookup
+      (fun yout =>
+         tspec
+           (withSpace
+              match yout, lookup x xs with
+              | true, Some y => SpecVector [|Contains _ xs; Contains _ y; Void; Void; Void|]
+              | false,  None => SpecVector [|Contains _ xs; Contains _ x; Void; Void; Void|]
+              | _, _ => SpecFalse
+              end (appSize (Lookup_size xs x) ss))).
+  Proof.
+    unfold Lookup. hsteps_cbn; cbn.
+    apply CopyValue_SpecT_size with (X := list (X*Y)).
+    cbn. apply Lookup_Loop_SpecT_space.
+    intros yout tout H. cbn in *.
+    destruct yout, (lookup x xs); cbn in *; eauto.
+    reflexivity.
+  Qed.
+
+  (* Legacy Lemma *)
+  Lemma Lookup_Realise : Lookup ⊨ Lookup_Rel.
+  Proof.
+    repeat (eapply RealiseIntroAll;intro). eapply Realise_monotone.
+    -eapply TripleT_Realise, (Lookup_SpecT_space x x0 [|x1;x2;x3;x4;x5|]).
+    -intros ? [] H **. modpon H.
+    {unfold "≃≃",withSpace;cbn. intros i; destruct_fin i;cbn. all:assumption. }
+    repeat destruct _;unfold "≃≃",withSpace in H;cbn in H.
+    2,3:contradiction.
+    all:specializeFin H;tauto.
+  Qed.
 
   Definition Lookup_T : tRel sig^+ 5 :=
     fun tin k =>
@@ -323,23 +247,22 @@ Section LookupAssociativeList.
         isVoid tin[@Fin2] /\ isVoid tin[@Fin3] /\ isVoid tin[@Fin4] /\
         Lookup_steps x xs <= k.
 
+  (* legacy Lemma *)
   Lemma Lookup_Terminates : projT1 Lookup ↓ Lookup_T.
   Proof.
-    eapply TerminatesIn_monotone.
-    { unfold Lookup. TM_Correct.
-      - apply CopyValue_Realise with (X := list (X*Y)).
-      - apply CopyValue_Terminates with (X := list (X*Y)).
-      - apply Lookup_Loop_Terminates. }
-    {
-      intros tin k (xs&x&HEncXs&HEncX&HRight2&HRight3&HRight4&Hk). unfold Lookup_steps in Hk.
-      exists (CopyValue_steps xs), (Lookup_Loop_steps x xs). repeat split; try lia.
-      { hnf. eauto. }
-      intros tmid [] (HCopy&HCopyInj); TMSimp. modpon HCopy.
-      cbn. hnf. do 2 eexists; repeat split; cbn; eauto.
-    }
+    repeat (eapply TerminatesInIntroEx;intro). eapply TerminatesIn_monotone.
+    -eapply TripleT_TerminatesIn. eapply TripleT_RemoveSpace,Lookup_SpecT_space.
+    -intros ? k H **. modpon H.
+    split. 2:eassumption. 
+    unfold "≃≃",withSpace;cbn. intros i; destruct_fin i;cbn. all:assumption. 
   Qed.
 
 End LookupAssociativeList.
 
 Arguments Lookup_steps {sigX sigY X Y cX cY} : simpl never.
 Arguments Lookup_size {sigX sigY X Y cX cY} : simpl never.
+
+Ltac hstep_LookupAssociativeList :=
+  match goal with
+  | [ |- TripleT ?P ?k (Lookup _ _) ?Q ] => eapply Lookup_SpecT_space
+  end.
